symlink + truncate

examples/fs/filesys.s.dfy
@@ -9,7 +9,6 @@ include "../../lib/Base/Sequences.i.dfy"
 
 module FileSys {
   import opened FileSysTypes
-  import opened Options
   import opened Sequences
 
   const DefaultId := -1;
@@ -56,11 +55,10 @@ module FileSys {
   predicate ValidNewPath(fs: FileSys, path: Path)
   requires WF(fs)
   {
-    && ValidPath(fs, path)
-    // parentdir checks
     && var parentdir := GetParentDir(path);
     && ValidPath(fs, parentdir)
-    && fs.meta_map[fs.path_map[parentdir]].stat.ftype.Directory?
+    && fs.meta_map[fs.path_map[parentdir]].ftype.Directory?
+    && fs.path_map[path] == DefaultId
   }
 
   predicate IsEmptyDir(fs: FileSys, dir: Path)
@@ -70,53 +68,51 @@ module FileSys {
     && (forall k | k != dir && IsPrefix(dir, k) && k[|dir|] as int == '/' as int :: fs.path_map[k] == DefaultId)
   }
 
-  predicate ValidNewStat(stat: Stat)
+  predicate ValidNewMetaData(m: MetaData)
   {
-    && stat.atime == stat.ctime == stat.mtime
-    && stat.size == 0
-    && stat.nlink == 1
+    && m.atime == m.ctime == m.mtime
+    && m.size == 0
+    && m.nlink == 1
   }
 
   // FileSys Ops
 
-  predicate GetAttr(fs: FileSys, fs':FileSys, path: Path, attr: Stat)
+  predicate GetAttr(fs: FileSys, fs':FileSys, path: Path, attr: MetaData)
   {
     && WF(fs)
     && ValidPath(fs, path)
     && fs' == fs
-    && attr == fs.meta_map[fs.path_map[path]].stat
+    && attr == fs.meta_map[fs.path_map[path]]
   }
 
-  predicate ReadLink(fs: FileSys, fs':FileSys, path: Path, link_path: Option<Path>)
+  predicate ReadLink(fs: FileSys, fs':FileSys, path: Path, link_path: Path)
   {
     && WF(fs)
     && ValidPath(fs, path)
     && fs' == fs
-    && link_path == fs.meta_map[fs.path_map[path]].source
+    && fs.meta_map[fs.path_map[path]].ftype.SymLink?
+    && link_path == fs.meta_map[fs.path_map[path]].ftype.source
   }
 
-  predicate Create(fs: FileSys, fs':FileSys, path: Path, id: int, stat: Stat)
+  predicate Create(fs: FileSys, fs':FileSys, path: Path, id: int, m: MetaData)
   {
     && WF(fs)
     && WF(fs')
     && ValidNewPath(fs, path)
-    && ValidNewStat(stat)
+    && ValidNewMetaData(m)
     && id != DefaultId
     // Entry Not Present
-    && fs.path_map[path] == DefaultId // Inv should make sure defaultId implies empty content
     && fs.meta_map[id] == EmptyMetaData() // implies id hasn't shown up
     && fs.data_map[id] == EmptyData()
     // Updated maps
     && fs'.path_map[path] == id
-    && fs'.meta_map == fs.meta_map[id := MetaData(stat, None)]
+    && fs'.meta_map == fs.meta_map[id := m]
     && fs'.data_map == fs.data_map
   }
 
   function MetaDataUpdateLink(m: MetaData, delta: int, ctime: Time): MetaData
   {
-    var newstat := Stat(m.stat.nlink+delta, m.stat.size, m.stat.ftype, m.stat.perm,
-        m.stat.uid, m.stat.gid, m.stat.atime, m.stat.mtime, ctime);
-    MetaData(newstat, m.source)
+    MetaData(m.nlink+delta, m.size, m.ftype, m.perm, m.uid, m.gid, m.atime, m.mtime, ctime)
   }
 
   predicate Delete(fs: FileSys, fs':FileSys, path: Path, ctime: Time)
@@ -125,30 +121,31 @@ module FileSys {
     && WF(fs')
     && ValidPath(fs, path)
     && var id := fs.path_map[path];
-    && (fs.meta_map[id].stat.ftype.Directory? ==> IsEmptyDir(fs, path))
+    && (fs.meta_map[id].ftype.Directory? ==> IsEmptyDir(fs, path))
     // maps after delete
     && fs'.path_map == fs.path_map[path := DefaultId]
-    && (fs.meta_map[id].stat.nlink == 1 ==> 
+    && (fs.meta_map[id].nlink == 1 ==> 
         && fs'.meta_map == fs.meta_map[id := EmptyMetaData()]
         && fs'.data_map == fs.data_map[id := EmptyData()])
-    && (fs.meta_map[id].stat.nlink > 1 ==> 
+    && (fs.meta_map[id].nlink > 1 ==> 
         && fs'.meta_map == fs.meta_map[id := MetaDataUpdateLink(fs.meta_map[id], -1, ctime)]
         && fs'.data_map == fs.data_map)
   }
 
-  // symlink_map: key = created symlink file, value = source file
-  // maybe we don't want to pass in a map
-  predicate SymLink(fs: FileSys, fs':FileSys, symlink_map: imap<Path, Path>)
+  predicate SymLink(fs: FileSys, fs':FileSys, source: Path, dest: Path, id: int, m: MetaData)
   {
     && WF(fs)
     && WF(fs')
-    && (forall k | k in symlink_map :: ValidNewPath(fs, k) && ValidPath(fs, path_map[k]))
+    && ValidNewPath(fs, dest) // source doesn't need to be valid
+    && ValidNewMetaData(m)
+    && m.ftype == FileType.SymLink(source)
+    && id != DefaultId
+    && fs.meta_map[id] == EmptyMetaData()
+    && fs.data_map[id] == EmptyData()
     // updated maps
-
-    // needs more thoughts: when we stat symlinked dir file we want to get to 
-    // && (forall k | k in symlink_map :: )
-
-    // TODO
+    && fs'.path_map == fs.path_map[dest := id]
+    && fs'.meta_map == fs.meta_map[id := m]
+    && fs'.data_map == fs.data_map
   }
 
   // rename is a map because we allow directory
@@ -166,7 +163,7 @@ module FileSys {
     && ValidPath(fs, source)  // NOTE: won't work for hardlink other filesystem files
     && ValidNewPath(fs, dest)
     && var id := fs.path_map[source];
-    && !fs.meta_map[id].stat.ftype.Directory?  // disallow directory hardlinks
+    && !fs.meta_map[id].ftype.Directory?  // disallow directory hardlinks
     // updated maps
     && fs'.path_map == fs.path_map[dest := id]
     && fs'.meta_map == fs.meta_map[id := MetaDataUpdateLink(fs.meta_map[id], 1, ctime)]
@@ -175,9 +172,7 @@ module FileSys {
 
   function MetaDataChangeAttr(m: MetaData, perm: int, uid:int, gid: int, ctime: Time): MetaData
   {
-    var newstat := Stat(m.stat.nlink, m.stat.size, m.stat.ftype, 
-      perm, uid, gid, m.stat.atime, m.stat.mtime, ctime);
-    MetaData(newstat, m.source)
+    MetaData(m.nlink, m.size, m.ftype, perm, uid, gid, m.atime, m.mtime, ctime)
   }
 
   // chown + chmod
@@ -192,13 +187,39 @@ module FileSys {
     && fs'.data_map == fs.data_map
   }
 
-  predicate Truncate(fs: FileSys, fs':FileSys, path: Path, size: int)
+  function MetaDataTruncate(m: MetaData, size: int, time: Time): MetaData
+  {
+    MetaData(m.nlink, size, m.ftype, m.perm, m.uid, m.gid, m.atime, time, time)
+  }
+
+  function ZeroData(size: int) : (d: Data)
+  requires size >= 0
+  ensures size == |d|
+  ensures forall i | 0 <= i < |d| :: d[i] == 0
+  {
+    if size == 0 then [] else ZeroData(size-1) + [0]
+  }
+
+  function DataTruncate(d: Data, size: int): (d': Data)
+  requires 0 <= size
+  ensures |d'| == size
+  {
+    if |d| >= size then d[..size] else d + ZeroData(size-|d|)
+  }
+
+  predicate Truncate(fs: FileSys, fs':FileSys, path: Path, size: int, time: Time)
   {
     && WF(fs)
     && WF(fs')
-    // truncate can go up or down, specify behavior accordingly
-    // what about special files?
-    // TODO
+    && 0 <= size
+    && ValidPath(fs, path)
+    && var id := fs.path_map[path];
+    && fs.meta_map[id].ftype.File?
+    && size != fs.meta_map[id].size
+    // updated maps
+    && fs'.path_map == fs.path_map
+    && fs'.meta_map == fs.meta_map[id := MetaDataTruncate(fs.meta_map[id], size, time)]
+    && fs'.data_map == fs.data_map[id := DataTruncate(fs.data_map[id], size)]
   }
 
   predicate Read(fs: FileSys, fs':FileSys, path: Path, offset: int, size: int, data: Data)
@@ -207,18 +228,16 @@ module FileSys {
     && fs' == fs
     && ValidPath(fs, path)
     && var id := fs.path_map[path];
-    && fs.meta_map[id].stat.ftype.File?
-    && fs.meta_map[id].source.None?
-    && 0 <= offset <= offset+size <= fs.meta_map[id].stat.size
-    && fs.meta_map[id].stat.size == |fs.data_map[id]|
+    && fs.meta_map[id].ftype.File?
+    && 0 <= offset <= offset+size <= fs.meta_map[id].size
+    && fs.meta_map[id].size == |fs.data_map[id]| // consistency
     && data == fs.data_map[id][offset..offset+size]
   }
 
   function MetaDataWrite(m: MetaData, newsize: int, time: Time): MetaData
   {
-    var size := if m.stat.size > newsize then m.stat.size else newsize;
-    var stat := Stat(m.stat.nlink, size, m.stat.ftype, m.stat.perm, m.stat.uid, m.stat.gid, time, time, time);
-    MetaData(stat, m.source)
+    var size := if m.size > newsize then m.size else newsize;
+    MetaData(m.nlink, size, m.ftype, m.perm, m.uid, m.gid, time, time, time)
   }
 
   function DataWrite(d: Data, data: Data, offset: int, size: int): (d': Data)
@@ -237,10 +256,9 @@ module FileSys {
     && ValidPath(fs, path)
     && |data| == size
     && var id := fs.path_map[path];
-    && fs.meta_map[id].stat.ftype.File?
-    && fs.meta_map[id].source.None?
-    && fs.meta_map[id].stat.size == |fs.data_map[id]|
-    && 0 <= offset <= fs.meta_map[id].stat.size 
+    && fs.meta_map[id].ftype.File?
+    && fs.meta_map[id].size == |fs.data_map[id]|
+    && 0 <= offset <= fs.meta_map[id].size
     // updated maps
     && fs'.path_map == fs.path_map
     && fs'.meta_map == fs.meta_map[id := MetaDataWrite(fs.meta_map[id], offset+size, time)]
@@ -249,9 +267,7 @@ module FileSys {
 
   function MetaDataUpdateTime(m: MetaData, atime: Time, mtime: Time, ctime: Time): MetaData
   {
-    var newstat := Stat(m.stat.nlink, m.stat.size, m.stat.ftype, 
-      m.stat.perm, m.stat.uid, m.stat.gid, atime, mtime, ctime);
-    MetaData(newstat, m.source)
+    MetaData(m.nlink, m.size, m.ftype, m.perm, m.uid, m.gid, atime, mtime, ctime)
   } 
 
   predicate UpdateTime(fs: FileSys, fs':FileSys, path: Path, atime: Time, mtime: Time, ctime: Time)
@@ -279,62 +295,35 @@ module FileSys {
   }
 
   datatype Step =
-    | GetAttrStep(path: Path, attr: Stat)
-    | ReadLinkStep(path: Path, link_path: Option<Path>)
-    | CreateStep(path: Path, id: int, stat: Stat) // mknod and mkdir
+    | GetAttrStep(path: Path, attr: MetaData)
+    | ReadLinkStep(path: Path, link_path: Path)
+    | CreateStep(path: Path, id: int, m: MetaData) // mknod and mkdir
     | DeleteStep(path: Path, ctime: Time) // unlink and rmdir
-    | SymLinkStep(symlink_map: imap<Path, Path>) // how to? path vs map? path: Path, link_path: Path
+    | SymLinkStep(source: Path, dest: Path, id: int, m: MetaData) // how to? path vs map? path: Path, link_path: Path
     | RenameStep(rename_map: imap<Path, Path>, flags: int) // a map of path to renames?
     | LinkStep(source: Path, dest: Path, ctime: Time)
     | ChangeAttrStep(path: Path, perm: int, uid: int, gid: int, ctime: Time) // chmod + chown
-    // | ChmodStep(path: Path, perm: int, ctime: Time)
-    // | ChownStep(path: Path, uid: int, gid: int)
-    | TruncateStep(path: Path, size: int)
+    | TruncateStep(path: Path, size: int, time: Time)
     | ReadStep(path: Path, offset: int, size: int, data: Data)
     | WriteStep(path: Path, offset: int, size: int, data: Data, time: Time)
-  //  | StatfsStep(fsstat: StatFS) // syscall param also has a path that points to any file of the fs
     | UpdateTimeStep(path: Path, atime: Time, mtime: Time, ctime: Time) 
     | ReadDirStep(path: Path) // TODO: fill in rest of params: starting entry, end as we stop seeing one with prefix
     | StutterStep
-  
-    /*
-      | MknodStep(path: Path, mode: Mode, rdev_id: int) // will have entry in data map
-      | MkdirStep(path: Path, mode: Mode) // only entry in metadata
-      | UnlinkStep(path: Path) // remove a file
-      | RmdirStep(path: Path)
-      | OpenStep(path: Path) 
-        // should open be a filesys spec? Does filesys need to encode permission checking if it's done by vfs?
-      | FlushStep(path: Path) skipped as it doesn't change the filesys?
-      | ReleaseStep(path: Path)
-      | FSyncStep(path: Path) // skipped here
-      | OpenDirStep(path: Path)
-      | ReleaseDirStep(path: Path)
-      | FSyncDir()
-      | DestroyFS // should this exist?
-      | SetXattrStep()
-      | GetXattrStep()
-      | ListXattrStep()
-      | RemoveXattrStep()
-
-      ignored fuse_ops:
-        access (relying on kernel vfs), create (create + open), destroy (clean up a filesys), lock (flock), 
-        bmap (map inode # to blk #), fallocate and so on
-    */
 
   predicate NextStep(fs: FileSys, fs': FileSys, step:Step)
   {
     match step {
       case GetAttrStep(path, attr) => GetAttr(fs, fs', path, attr)
       case ReadLinkStep(path, link_path) => ReadLink(fs, fs', path, link_path)
-      case CreateStep(path, id, stat) => Create(fs, fs', path, id, stat)
+      case CreateStep(path, id, m) => Create(fs, fs', path, id, m)
       case DeleteStep(path, ctime) => Delete(fs, fs', path, ctime)
-      case SymLinkStep(symlink_map) => SymLink(fs, fs', symlink_map)
+      case SymLinkStep(source, dest, id, m) => SymLink(fs, fs', source, dest, id, m)
       case RenameStep(rename_map, flags) => Rename(fs, fs', rename_map, flags)
       case LinkStep(source, dest, ctime) => Link(fs, fs', source, dest, ctime)
       case ChangeAttrStep(path, perm, uid, gid, ctime) => ChangeAttr(fs, fs', path, perm, uid, gid, ctime)
       // case ChmodStep(path, mode, ctime) => Chmod(fs, fs', path, mode, ctime)
       // case ChownStep(path, uid, gid) => Chown(fs, fs', path, uid, gid)
-      case TruncateStep(path, size) => Truncate(fs, fs', path, size)
+      case TruncateStep(path, size, time) => Truncate(fs, fs', path, size, time)
       case ReadStep(path, offset, size, data) => Read(fs, fs', path, offset, size, data)
       case WriteStep(path, offset, size, data, time) => Write(fs, fs', path, offset, size, data, time)
       case UpdateTimeStep(path, atime, mtime, ctime) => UpdateTime(fs, fs', path, atime, mtime, ctime)
@@ -378,5 +367,30 @@ module FileSys {
   lemma NextPreservesInv(fs: FileSys, fs': FileSys) // add ui op
   {
   }
+
+   
+    /*
+      | MknodStep(path: Path, mode: Mode, rdev_id: int) // will have entry in data map
+      | MkdirStep(path: Path, mode: Mode) // only entry in metadata
+      | UnlinkStep(path: Path) // remove a file
+      | RmdirStep(path: Path)
+      | OpenStep(path: Path) 
+      | FlushStep(path: Path) skipped as it doesn't change the filesys?
+      | ReleaseStep(path: Path)
+      | FSyncStep(path: Path) // skipped here
+      | OpenDirStep(path: Path)
+      | ReleaseDirStep(path: Path)
+      | FSyncDir()
+      | DestroyFS // should this exist?
+      | SetXattrStep()
+      | GetXattrStep()
+      | ListXattrStep()
+      | RemoveXattrStep()
+
+      ignored fuse_ops:
+        access (relying on kernel vfs), create (create + open), destroy (clean up a filesys), lock (flock), 
+        bmap (map inode # to blk #), fallocate and so on
+    */
+
 
 }
